src/FS/SepLogic/Pred/Except.v
@@ -8,6 +8,9 @@ Require Import FS.SepLogic.Pred.Def.
 Definition pred_except `(F: pred A V) {AEQ: EqDec A eq} a v : pred A V :=
   mkPred (fun m => upd m a v |= F).
 
+Definition pred_eexcept `(F: pred A V) {AEQ: EqDec A eq} a : pred A V :=
+  mkPred (fun m => exists v, upd m a v |= F).
+
 Definition mem_except `(m: mem A V) {AEQ: EqDec A eq} a : mem A V :=
   fun a' => if a == a' then None
          else m a'.
@@ -29,3 +32,11 @@ Proof.
   rewrite H3; auto.
 *)
 Admitted.
+
+Axiom pred_eexcept_ptsto_eq : forall `(F: pred A V) {AEQ: EqDec A eq} a (v : V),
+  pred_eexcept (a |-> v) a ===> emp.
+Axiom pred_eexcept_ptsto_ne : forall `(F: pred A V) {AEQ: EqDec A eq} a' a (v : V),
+  a <> a' ->
+  pred_eexcept (a |-> v) a' ===> a |-> v.
+Axiom pred_eexcept_star : forall `(p1: pred A V) p2 {AEQ: EqDec A eq} a',
+  pred_eexcept (p1 * p2) a' ===> pred_eexcept p1 a' * pred_eexcept p2 a'.
