src/FS/SepLogic/Pred.v
@@ -4,5 +4,6 @@ Require Export
         FS.SepLogic.Pred.Impl
         FS.SepLogic.Pred.Except
         FS.SepLogic.Pred.MemIs
-        FS.SepLogic.Pred.MemIsExcept.
+        FS.SepLogic.Pred.MemIsExcept
+        FS.SepLogic.Pred.Cancel.
 Global Opaque pred_prop.
