src/FS/SepLogic/Pred/Cancel.v
@@ -1,0 +1,116 @@
+Require Import List.
+Require Import SepLogic.Pred.Def.
+Require Import SepLogic.Pred.Ptsto.
+Import ListNotations.
+
+
+Definition pred_fold_left `(l : list (pred A V)) : pred A V :=
+  match l with
+  | nil => emp
+  | a :: t => fold_left star t a
+  end.
+
+Definition stars `(ps : list (pred A V)) :=
+  pred_fold_left ps.
+Arguments stars : simpl never.
+
+
+Lemma flatten_emp : forall A V,
+  (@emp A V) === stars nil.
+Admitted.
+
+Lemma flatten_default : forall `(p : pred A V),
+  p === stars (p :: nil).
+Admitted.
+
+Lemma flatten_star : forall `(p : pred A V) q ps qs,
+  p === stars ps
+  -> q === stars qs
+  -> p * q === stars (ps ++ qs).
+Admitted.
+
+Ltac flatten :=
+  repeat match goal with
+  | [ |- emp === _ ] => apply flatten_emp
+  | [ |- _ * _ === _ ] => eapply flatten_star
+  | _ => apply flatten_default
+  end.
+
+Example flatten1 : forall `(p : pred A V) q r s t u, exists l, p * q * r * (s * t) * u === stars l /\ l = nil.
+Proof.
+  intros. eexists. split. flatten. simpl.
+Abort.
+
+
+Theorem start_normalizing_left : forall `(p : pred A V) q ps,
+  p === stars ps
+  -> ((stars ps * stars nil) ===> q)
+  -> p ===> q.
+Admitted.
+
+Theorem start_normalizing_right : forall `(p : pred A V) q qs,
+  q === stars qs
+  -> (p ===> stars qs)
+  -> p ===> q.
+Admitted.
+
+Ltac norml := eapply start_normalizing_left; [ flatten | ]; simpl app.
+Ltac normr := eapply start_normalizing_right; [ flatten | ]; simpl app.
+Ltac norm := norml; normr.
+
+Example norm1 : forall `(p : pred A V) q r s,
+  p * q * r * s ===> (p * q) * (s * r).
+Proof.
+  intros.
+  norm.
+Abort.
+
+
+Definition okToUnify `(p1 : pred A V) p2 := p1 = p2.
+Hint Extern 0 (okToUnify ?a ?a) => constructor : okToUnify.
+Hint Extern 0 (okToUnify (ptsto ?p _) (ptsto ?p _)) => constructor : okToUnify.
+
+
+Inductive pick {A V} (lhs : pred A V) : list (pred A V) -> list (pred A V) -> Prop :=
+| PickFirst : forall p ps,
+  okToUnify lhs p
+  -> pick lhs (p :: ps) ps
+| PickLater : forall p ps ps',
+  pick lhs ps ps'
+  -> pick lhs (p :: ps) (p :: ps').
+
+Ltac pick :=
+  solve [ repeat
+          ( (apply PickFirst; solve [ trivial with okToUnify ]) ||
+            apply PickLater ) ].
+
+
+Theorem cancel_one : forall `(p : pred A V) qs qs' ps F,
+  pick p qs qs'
+  -> stars ps * F ===> stars qs'
+  -> stars (p :: ps) * F ===> stars qs.
+Admitted.
+
+Theorem delay_one : forall `(p : pred A V) ps q qs,
+  stars ps * stars (p :: qs) ===> q
+  -> stars (p :: ps) * stars qs ===> q.
+Admitted.
+
+Ltac cancel_one := eapply cancel_one; [ pick | ].
+Ltac delay_one := apply delay_one.
+Ltac cancel := repeat ( cancel_one || delay_one ).
+
+
+Lemma cancel_finish : forall A V,
+  @stars A V [] * stars [] ===> stars [].
+Admitted.
+
+Ltac cancel_finish := apply cancel_finish.
+
+
+Example cancel1 : forall `(p : pred A V) q r s,
+  p * q * r * s ===> (p * q) * (s * r).
+Proof.
+  intros.
+  norm. cancel. cancel_finish.
+Qed.
